Convert StatDB example to Module format.

src/Examples/ExMach/RefinementAdequacy.v
@@ -28,77 +28,101 @@ Module Type exmach_refinement_type.
   Context (crash_starter: forall {H1 : @cfgG OpT Λa Σ} {H2 : exmachG Σ},
               @crash_param _ H2 → iProp Σ).
   Context (exec_inv: forall {_ : @cfgG OpT Λa Σ} {_ : exmachG Σ}, iProp Σ).
-  Context (einv_persist: forall {H1 : @cfgG OpT Λa Σ} {H2 : _},
-              Persistent (exec_inv H1 H2)).
-  Context (cinv_persist: forall {H1 : @cfgG OpT Λa Σ} {H2 : _}
-            {P: crash_param _ _}, Persistent (crash_inv H1 H2 P)).
 
   Context (E: coPset).
-  Context (nameIncl: nclose sourceN ⊆ E).
   (* TODO: we should get rid of rec_seq if we're not exploiting vertical comp anymore *)
   Context (recv: proc ExMach.Op unit).
-  Context (recsingle: recover = rec_singleton recv).
+  Context (init_absr: Λa.(OpState) → ExMach.State → Prop).
+End exmach_refinement_type.
 
-  Context (refinement_op_triples:
-             forall {H1 H2 T1 T2} j K `{LanguageCtx OpT T1 T2 Λa K} (op: OpT T1),
-               j ⤇ K (Call op) ∗ Registered ∗ (@exec_inv H1 H2) ⊢
-                 WP compile (Call op) {{ v, j ⤇ K (Ret v) ∗ Registered  }}).
+Module exmach_refinement_definitions (eRT: exmach_refinement_type).
+  Import eRT.
 
-  Context (exec_inv_source_ctx: ∀ {H1 H2}, exec_inv H1 H2 ⊢ source_ctx).
-
-  Context (recv_triple:
+  Definition recv_triple_type :=
              forall {H1 H2} param,
                (@crash_inv H1 H2 param) ∗ Registered ∗ (@crash_starter H1 H2 param) ⊢
                     WP recv @ NotStuck; ⊤ {{ v, |={⊤,E}=> ∃ σ2a σ2a', source_state σ2a
                     ∗ ⌜Λa.(crash_step) σ2a (Val σ2a' tt)⌝ ∗
                     ∀ `{Hcfg': cfgG OpT Λa Σ} (Hinv': invG Σ) tr',
-                      source_ctx ∗ source_state σ2a'  ={⊤}=∗
+                      source_ctx ∗ source_state σ2a' ={⊤}=∗
                       exec_inner Hcfg' (ExMachG Σ Hinv' exm_mem_inG exm_disk_inG tr')
-                                               }}).
+                                               }}.
+  Definition refinement_op_triples_type :=
+             forall {H1 H2 T1 T2} j K `{LanguageCtx OpT T1 T2 Λa K} (op: OpT T1),
+               j ⤇ K (Call op) ∗ Registered ∗ (@exec_inv H1 H2) ⊢
+                 WP compile (Call op) {{ v, j ⤇ K (Ret v) ∗ Registered  }}.
 
-  Context (init_absr: Λa.(OpState) → ExMach.State → Prop).
-  Context (init_wf: ∀ σ1a σ1c, init_absr σ1a σ1c → state_wf σ1c).
 
-  Context (init_exec_inner: ∀ σ1a σ1c, init_absr σ1a σ1c →
+  Definition init_exec_inner_type :=
+    ∀ σ1a σ1c, init_absr σ1a σ1c →
       (∀ `{Hex: exmachG Σ} `{Hcfg: cfgG OpT Λa Σ},
           (([∗ map] i ↦ v ∈ mem_state σ1c, i m↦ v) ∗
            ([∗ map] i ↦ v ∈ disk_state σ1c, i d↦ v) ∗
-           source_ctx ∗ source_state σ1a) ={⊤}=∗ exec_inner _ _)).
+           source_ctx ∗ source_state σ1a) ={⊤}=∗ exec_inner _ _).
 
-  Context (exec_inv_preserve_crash:
+  Definition exec_inv_preserve_crash_type :=
       (∀ `{Hex: exmachG Σ} `{Hcfg: cfgG OpT Λa Σ},
           exec_inv Hcfg Hex ={⊤, E}=∗ ∀ Hmem' Hreg',
           (let Hex := ExMachG Σ (exm_invG) Hmem' (exm_disk_inG) Hreg' in
-              ([∗ map] i ↦ v ∈ init_zero, i m↦ v) ={E}=∗ crash_inner Hcfg Hex))).
+              ([∗ map] i ↦ v ∈ init_zero, i m↦ v) ={E}=∗ crash_inner Hcfg Hex)).
 
-  Context (crash_inv_preserve_crash:
+  Definition crash_inv_preserve_crash_type :=
       (∀ `{Hex: exmachG Σ} `{Hcfg: cfgG OpT Λa Σ} param,
           crash_inv Hcfg Hex param ={⊤, E}=∗ ∀ Hmem' Hreg',
           (let Hex := ExMachG Σ (exm_invG) Hmem' (exm_disk_inG) Hreg' in
-              ([∗ map] i ↦ v ∈ init_zero, i m↦ v) ={E}=∗ crash_inner Hcfg Hex))).
+              ([∗ map] i ↦ v ∈ init_zero, i m↦ v) ={E}=∗ crash_inner Hcfg Hex)).
 
-  Context (crash_inner_inv :
+  Definition crash_inner_inv_type :=
       (∀ `{Hex: exmachG Σ} `{Hcfg: cfgG OpT Λa Σ},
           (∃ Hinv, crash_inner Hcfg (ExMachG Σ Hinv (exm_mem_inG) (exm_disk_inG) (exm_treg_inG))) ∗
-          source_ctx ={⊤}=∗ ∃ param, crash_inv Hcfg Hex param ∗ crash_starter Hcfg Hex param)).
+          source_ctx ={⊤}=∗ ∃ param, crash_inv Hcfg Hex param ∗ crash_starter Hcfg Hex param).
 
-  Context (exec_inner_inv :
+  Definition exec_inner_inv_type :=
       (∀ `{Hex: exmachG Σ} `{Hcfg: cfgG OpT Λa Σ},
           (∃ Hinv, exec_inner Hcfg (ExMachG Σ Hinv (exm_mem_inG) (exm_disk_inG) (exm_treg_inG))) ∗
-          source_ctx ={⊤}=∗ exec_inv Hcfg Hex)).
+          source_ctx ={⊤}=∗ exec_inv Hcfg Hex).
 
-  Context (exec_inv_preserve_finish:
+  Definition exec_inv_preserve_finish_type :=
       (∀ `{Hex: exmachG Σ} `{Hcfg: cfgG OpT Λa Σ},
           AllDone -∗ exec_inv Hcfg Hex ={⊤, E}=∗ ∃ (σ2a σ2a' : Λa.(OpState)), source_state σ2a
           ∗ ⌜Λa.(finish_step) σ2a (Val σ2a' tt)⌝ ∗
           ∀ `{Hcfg': cfgG OpT Λa Σ} (Hinv': invG Σ) Hmem' Hreg',
             (let Hex := ExMachG Σ Hinv' Hmem' (exm_disk_inG) Hreg' in
             source_ctx∗ source_state σ2a' ∗ ([∗ map] i ↦ v ∈ init_zero, i m↦ v) ={⊤}=∗
-               exec_inner Hcfg' Hex))%I).
+               exec_inner Hcfg' Hex))%I.
 
-End exmach_refinement_type.
+End exmach_refinement_definitions.
 
-Module exmach_refinement (eRT: exmach_refinement_type).
+
+
+Module Type exmach_refinement_obligations (eRT: exmach_refinement_type).
+
+  Module eRD := exmach_refinement_definitions eRT.
+  Import eRT.
+  Import eRD.
+
+  Context (recsingle: recover = rec_singleton eRT.recv).
+
+  Context (nameIncl: nclose sourceN ⊆ eRT.E).
+  Context (einv_persist: forall {H1 : @cfgG OpT Λa eRT.Σ} {H2 : _},
+              Persistent (exec_inv H1 H2)).
+  Context (cinv_persist: forall {H1 : @cfgG OpT Λa Σ} {H2 : _}
+            {P: crash_param _ _}, Persistent (crash_inv H1 H2 P)).
+
+  Context (exec_inv_source_ctx: ∀ {H1 H2}, exec_inv H1 H2 ⊢ source_ctx).
+
+  Context (recv_triple: recv_triple_type).
+  Context (init_wf: ∀ σ1a σ1c, init_absr σ1a σ1c → state_wf σ1c).
+  Context (refinement_op_triples: refinement_op_triples_type).
+  Context (init_exec_inner: init_exec_inner_type).
+  Context (exec_inv_preserve_crash: exec_inv_preserve_crash_type).
+  Context (crash_inv_preserve_crash: crash_inv_preserve_crash_type).
+  Context (exec_inner_inv: exec_inner_inv_type).
+  Context (crash_inner_inv: crash_inner_inv_type).
+  Context (exec_inv_preserve_finish : exec_inv_preserve_finish_type).
+End exmach_refinement_obligations.
+
+Module exmach_refinement (eRT: exmach_refinement_type) (eRO: exmach_refinement_obligations eRT).
 
   Module RT <: refinement_type.
     Import eRT.
@@ -125,16 +149,9 @@ Module exmach_refinement (eRT: exmach_refinement_type).
     Definition crash_param := crash_param.
     Definition crash_starter := crash_starter.
     Definition exec_inv := exec_inv.
-    Definition einv_persist := einv_persist.
-    Definition cinv_persist := cinv_persist.
     Definition E := E.
-    Definition nameIncl := nameIncl.
     Definition recv := recv.
-    Definition recsingle := recsingle.
-    Definition refinement_op_triples := refinement_op_triples.
-    Definition exec_inv_source_ctx := exec_inv_source_ctx.
     Definition init_absr := init_absr.
-
 
   End RT.
 
@@ -146,6 +163,15 @@ Module exmach_refinement (eRT: exmach_refinement_type).
     Module RD := RD.
     Import WeakestPre.
     Import RT RD.
+
+    Definition nameIncl := eRO.nameIncl.
+    Definition einv_persist := eRO.einv_persist.
+    Definition cinv_persist := eRO.cinv_persist.
+    Existing Instances einv_persist cinv_persist.
+    Definition recsingle := eRO.recsingle.
+    Definition refinement_op_triples := eRO.refinement_op_triples.
+    Definition exec_inv_source_ctx := eRO.exec_inv_source_ctx.
+
 
     Lemma set_inv_reg_spec0:
              ∀ Hex, (set_inv_reg Hex (Hinstance Σ Hex).(@iris_invG OpC (State Λc) Σ)
@@ -170,14 +196,13 @@ Module exmach_refinement (eRT: exmach_refinement_type).
                                      -∗ thread_count_interp n ∗ Interp σ) ∧
                 ∀ n σ, thread_count_interp n ∗ Interp σ -∗ state_interp (n, σ).
     Proof. eexists. split; eauto using thread_reg1, thread_reg2. Qed.
-    Definition refinement_op_triples := refinement_op_triples.
 
     (* This is just to convert from the old recv_triple style to the new one. *)
     Lemma recv_triple : recv_triple_type.
     Proof.
       rewrite /recv_triple_type.
       iIntros (???) "(#Hinv&Hreg&Hstart)".
-      iPoseProof @eRT.recv_triple as "H".
+      iPoseProof @eRO.recv_triple as "H".
       iSpecialize ("H" with "[$]").
       iApply (wp_wand with "H").
       iIntros (_) "H".
@@ -196,7 +221,7 @@ Module exmach_refinement (eRT: exmach_refinement_type).
       iIntros (σ1a σ1c Hinit ???).
       iMod (gen_heap_strong_init (mem_state σ1c)) as (hM Hmpf_eq) "(Hmc&Hm)".
       iMod (gen_heap_strong_init (disk_state σ1c)) as (hD Hdpf_eq) "(Hdc&Hd)".
-      iPoseProof (eRT.init_exec_inner σ1a σ1c Hinit (ExMachG Σ _ hM hD _) _) as "H".
+      iPoseProof (eRO.init_exec_inner σ1a σ1c Hinit (ExMachG Σ _ hM hD _) _) as "H".
       iModIntro. iExists (ExMachG Σ _ hM hD _). iIntros "(Hsource1&Hsource2&Hthread)".
       iMod ("H" with "[Hm Hd Hsource1 Hsource2]") as "Hinner".
       { iFrame.  iSplitL "Hm".
@@ -206,7 +231,7 @@ Module exmach_refinement (eRT: exmach_refinement_type).
       iFrame. simpl.
       iModIntro. iExists _, _. iFrame.
       iPureIntro;
-      edestruct (eRT.init_wf) as (Hwf1&Hwf2); eauto.
+      edestruct (eRO.init_wf) as (Hwf1&Hwf2); eauto.
       split_and!; eauto; intros i.
       * destruct (Hwf1 i); intuition.
       * destruct (Hwf2 i); intuition.
@@ -216,7 +241,7 @@ Module exmach_refinement (eRT: exmach_refinement_type).
   Proof.
     rewrite /exec_inv_preserve_crash_type.
     iIntros (??) "Hinv".
-    iPoseProof (eRT.exec_inv_preserve_crash with "Hinv") as "Hinv_post".
+    iPoseProof (eRO.exec_inv_preserve_crash with "Hinv") as "Hinv_post".
     iMod (gen_heap_strong_init (init_zero)) as (hM Hmpf_eq) "(Hmc&Hm)".
     iMod ("Hinv_post") as "Hinv_post".
     iModIntro. iIntros (?).
@@ -241,7 +266,7 @@ Module exmach_refinement (eRT: exmach_refinement_type).
   Proof.
     rewrite /crash_inv_preserve_crash_type.
     iIntros (???) "Hinv".
-    iPoseProof (eRT.crash_inv_preserve_crash with "Hinv") as "Hinv_post".
+    iPoseProof (eRO.crash_inv_preserve_crash with "Hinv") as "Hinv_post".
     iMod (gen_heap_strong_init (init_zero)) as (hM Hmpf_eq) "(Hmc&Hm)".
     iMod ("Hinv_post") as "Hinv_post".
     iModIntro. iIntros (?).
@@ -268,14 +293,14 @@ Module exmach_refinement (eRT: exmach_refinement_type).
   Lemma crash_inner_inv : crash_inner_inv_type.
   Proof.
     iIntros (??) "Hinner".
-    iPoseProof (eRT.crash_inner_inv with "Hinner") as "Hinv".
+    iPoseProof (eRO.crash_inner_inv with "Hinner") as "Hinv".
     eauto.
   Qed.
 
   Lemma exec_inner_inv : exec_inner_inv_type.
   Proof.
     iIntros (??) "Hinner".
-    iPoseProof (eRT.exec_inner_inv with "Hinner") as "Hinv".
+    iPoseProof (eRO.exec_inner_inv with "Hinner") as "Hinv".
     eauto.
   Qed.
 
@@ -283,7 +308,7 @@ Module exmach_refinement (eRT: exmach_refinement_type).
   Lemma exec_inv_preserve_finish : exec_inv_preserve_finish_type.
   Proof.
     iIntros (??) "Hdone Hinv".
-    iPoseProof (eRT.exec_inv_preserve_finish) as "H".
+    iPoseProof (eRO.exec_inv_preserve_finish) as "H".
     iMod ("H" $! _ _ with "[$] [$]") as (??) "(?&?&Hinv_post)".
     iModIntro. iExists _, _. iFrame. iIntros.
     iIntros (??? Hfinish ??) "((?&Hdisk)&?)".
@@ -312,7 +337,7 @@ Module exmach_refinement (eRT: exmach_refinement_type).
   Module R := refinement RT RO.
 
 
-  Export RO.
+  Export R.
 
 End exmach_refinement.
 
