src/Examples/StatDb/Refinement.v
@@ -110,129 +110,197 @@ Section refinement_triples.
 
 End refinement_triples.
 
-Section refinement.
+Module sRT <: exmach_refinement_type.
+
+
+  Definition OpT := DB.Op.
+  Definition Λa := DB.l.
 
   Definition helperΣ : gFunctors := #[GFunctor (authR (optionUR (exclR (listC natC))))].
   Instance subG_helperΣ : subG helperΣ Σ → inG Σ (authR (optionUR (exclR (listC natC)))).
   Proof. solve_inG. Qed.
 
-  Definition myΣ : gFunctors := #[Adequacy.exmachΣ; @cfgΣ DB.Op DB.l; lockΣ; helperΣ].
+  Definition Σ : gFunctors := #[Adequacy.exmachΣ; @cfgΣ DB.Op DB.l; lockΣ; helperΣ].
+  Definition impl := StatDb.Impl.impl.
   Existing Instance subG_cfgPreG.
+
+  Instance CFG : @cfgPreG DB.Op DB.l Σ. apply _. Qed.
+  Instance HEX : ExMach.Adequacy.exmachPreG Σ. apply _. Qed.
+  Instance INV : Adequacy.invPreG Σ. apply _. Qed.
+  Instance REG : inG Σ (csumR countingR (authR (optionUR (exclR unitC)))). apply _. Qed.
+
+  Definition crash_inner := fun H1 H2 => (@DBCrashInner Σ H2 H1)%I.
+  Definition exec_inner := fun (H1: @cfgG OpT Λa Σ) H2 => (∃ v, lock_addr m↦ v ∗
+            (∃ γ, (⌜ v = 0  ⌝-∗ @DBLockInv Σ H2 _ γ) ∗ @DBInnerInv _ _ _ γ))%I.
+  Definition crash_param := fun (_ : @cfgG OpT Λa Σ) (_ : exmachG Σ) => unit.
+  Definition crash_inv := fun H1 H2 (_ : crash_param _ _) => @CrashInv Σ H2 H1.
+  Definition crash_starter :=
+    fun H1 H2 (_ : crash_param H1 H2) => (True%I : iProp Σ).
+  Definition exec_inv := fun H1 H2 => (@DBInv Σ H2 _ H1 _)%I.
+  Definition E := nclose sourceN.
 
   Definition init_absr σ1a σ1c :=
     ExMach.l.(initP) σ1c ∧ DB.l.(initP) σ1a.
 
+  Definition recv: proc ExMach.Op unit := Ret tt.
 
-  Import ExMach.
-  Lemma exmach_crash_refinement_seq {T} σ1c σ1a (es: proc_seq DB.Op T) :
-    init_absr σ1a σ1c →
-    wf_client_seq es →
-    ¬ proc_exec_seq DB.l es (rec_singleton (Ret ())) (1, σ1a) Err →
-    ∀ σ2c res, proc_exec_seq ExMach.l (compile_proc_seq StatDb.Impl.impl es)
-                                        (rec_singleton recv) (1, σ1c) (Val σ2c res) →
-    ∃ σ2a, proc_exec_seq DB.l es (rec_singleton (Ret tt)) (1, σ1a) (Val σ2a res).
+End sRT.
+
+Module sRD := exmach_refinement_definitions sRT.
+
+Module sRO : exmach_refinement_obligations sRT.
+
+  Module eRD := exmach_refinement_definitions sRT.
+  Import sRT.
+  Import sRD.
+
+  Lemma einv_persist: forall {H1 : @cfgG OpT Λa Σ} {H2 : _},
+      Persistent (exec_inv H1 H2).
+  Proof. apply _. Qed.
+
+  Lemma cinv_persist: forall {H1 : @cfgG OpT Λa Σ} {H2 : _} P,
+      Persistent (crash_inv H1 H2 P).
+  Proof. apply _. Qed.
+
+  Lemma nameIncl: nclose sourceN ⊆ E.
+  Proof. solve_ndisj. Qed.
+
+  Lemma recsingle: recover impl = rec_singleton recv.
+  Proof. trivial. Qed.
+
+  Lemma refinement_op_triples: refinement_op_triples_type.
   Proof.
-    eapply (exmach_crash_refinement_seq) with
-        (Σ := myΣ)
-        (exec_inv := fun H1 H2 => (@DBInv myΣ H2 _ H1 _)%I)
-        (exec_inner := fun H1 H2 => (∃ v, lock_addr m↦ v ∗
-            (∃ γ, (⌜ v = 0  ⌝-∗ @DBLockInv myΣ H2 _ γ) ∗ @DBInnerInv _ _ _ γ))%I)
-        (crash_param := fun _ _ => unit)
-        (crash_inner := fun H1 H2 => (@DBCrashInner myΣ H2 H1)%I)
-        (crash_inv := fun H1 H2 _ => @CrashInv myΣ H2 H1)
-        (crash_starter := fun H1 H2 _ => True%I)
-        (E := nclose sourceN).
-    { apply _. }
-    { apply _. }
-    { intros. apply _. }
-    { intros. apply _. }
-    { set_solver+. }
-    { intros. iIntros "(?&?&HDB)". destruct op.
-      - iApply (add_refinement with "[$]"). iNext. iIntros (?) "H". iFrame.
-      - iApply (avg_refinement with "[$]"). iNext. iIntros (?) "H". iFrame.
-    }
-    { iIntros (??) "(?&?)"; eauto. }
-    { intros. iIntros "((#Hctx&#Hinv)&_&_)".
-      wp_ret. iInv "Hinv" as (l) ">(?&?&?&?)" "_".
-      rewrite /source_inv.
-      iMod (own_alloc (● (Excl' nil) ⋅ ◯ (Excl' nil))) as (γ2) "[Hauth Hfrag]".
-      { apply auth_both_valid; done. }
-      iApply (fupd_mask_weaken _ _).
-      { solve_ndisj. }
-      iExists l, nil. iFrame.
-      iSplitL "".
-      { iPureIntro; econstructor. }
-      iClear "Hctx Hinv".
-      iIntros (???) "(#Hctx&Hstate)".
-      rewrite /DBLockInv.
-      iModIntro. iExists _. iFrame. iExists γ2. iSplitR "Hauth Hstate"; iIntros; iExists nil; iFrame.
-    }
-    { intros ?? (H&?). inversion H. subst. eapply ExMach.init_state_wf. }
-    { intros ?? (H&Hinit) ??. inversion H. inversion Hinit. subst.
-      iIntros "(Hmem&?&#?&Hstate)".
-      iMod (own_alloc (● (Excl' nil) ⋅ ◯ (Excl' nil))) as (γ2) "[Hauth Hfrag]".
-      { apply auth_both_valid. split; done. }
-      iPoseProof (init_mem_split with "Hmem") as "(?&?&?)".
-      iModIntro. iExists _. iFrame. iExists γ2. iSplitR "Hauth Hstate"; iIntros; iExists nil; iFrame.
-    }
-    { intros. iIntros "(#Hctx&#Hinv)".
-      iDestruct "Hinv" as (γ1 γ2) "(Hlock&#Hinv)".
-      rewrite /DBCrashInner.
-      iInv "Hinv" as ">Hopen" "_".
-      iDestruct "Hopen" as (l) "(?&?)".
-      iApply fupd_mask_weaken; first by solve_ndisj.
-      iIntros (??) "Hmem".
-      iModIntro. iExists l; iFrame.
-      iPoseProof (@init_mem_split with "Hmem") as "(?&?&?)".
-      iFrame.
-    }
-    { intros. iIntros "(#Hctx&#Hinv)".
-      rewrite /DBCrashInner.
-      iInv "Hinv" as ">Hopen" "_".
-      iDestruct "Hopen" as (l) "(?&?)".
-      iApply fupd_mask_weaken; first by solve_ndisj.
-      iIntros (??) "Hmem".
-      iModIntro. iExists l. iFrame.
-      iPoseProof (@init_mem_split with "Hmem") as "(?&?&?)".
-      iFrame.
-    }
-    { intros. iIntros "H". iDestruct "H" as "(Hinv&#Hsrc)".
-      iDestruct "Hinv" as (invG) "Hinv".
-      rewrite /DBCrashInner/CrashInv.
-      iDestruct "Hinv" as (l) "(?&?)".
-      iMod (@inv_alloc myΣ (exm_invG) iN _ DBCrashInner with "[-]").
-      { iNext. iExists l; iFrame. }
-      iModIntro. iFrame. iExists tt. iFrame "Hsrc".
-    }
-    { intros. iIntros "H". iDestruct "H" as "(Hinv&#Hsrc)".
-      iDestruct "Hinv" as (invG v) "Hinv".
-      iDestruct "Hinv" as "(?&Hinv)".
-      iDestruct "Hinv" as (γ2) "(Hlock&Hinner)".
-      iMod (@lock_init myΣ (ExMachG _ (exm_invG) (exm_mem_inG) (exm_disk_inG) _) _ lN
-                       lock_addr _ (DBLockInv γ2) with "[$] [-Hinner]") as (γ1) "H".
-      { iFrame. }
-      iMod (@inv_alloc myΣ (exm_invG) iN _ (DBInnerInv γ2) with "[Hinner]").
-      { iFrame. }
-      iModIntro. rewrite /DBInv. iFrame "Hsrc". iExists γ1, γ2. iFrame.
-    }
-    { iIntros (??) "? (?&H)".
-      iDestruct "H" as (γ1 γ2) "(Hlock&Hinv)".
-      iInv "Hinv" as (l') ">(Htok&Hsource)" "_".
-      iMod (lock_crack with "Hlock") as ">H"; first by solve_ndisj.
-      iDestruct "H" as (v) "(?&?)".
-      iApply fupd_mask_weaken; first by solve_ndisj.
-      iExists _, nil; eauto.
-      iFrame. iSplitL ""; first by eauto.
-      iIntros (????) "(?&Hstate&Hmem)".
-      iPoseProof (@init_mem_split with "Hmem") as "(?&?&?)".
-      iMod (own_alloc (● (Excl' nil) ⋅ ◯ (Excl' nil))) as (γ2') "[Hauth Hfrag]".
-      { apply auth_both_valid. split; done. }
-      iModIntro. iExists O. iFrame.
-      iExists γ2'. rewrite /DBInnerInv/DBLockInv.
-      iSplitR "Hstate Hauth".
-      { iIntros. iExists _; iFrame. }
-      { iExists _; iFrame. }
-    }
+    rewrite /refinement_op_triples_type. intros. iIntros "(?&?&HDB)". destruct op.
+    - iApply (add_refinement with "[$]"). iNext. iIntros (?) "H". iFrame.
+    - iApply (avg_refinement with "[$]"). iNext. iIntros (?) "H". iFrame.
   Qed.
 
-End refinement.
+  Lemma exec_inv_source_ctx: ∀ {H1 H2}, exec_inv H1 H2 ⊢ source_ctx.
+  Proof. iIntros (??) "(?&?)"; eauto. Qed.
+
+  Lemma recv_triple: recv_triple_type.
+  Proof.
+    rewrite /recv_triple_type.
+    intros. iIntros "((#Hctx&#Hinv)&_&_)".
+    wp_ret. iInv "Hinv" as (l) ">(?&?&?&?)" "_".
+    rewrite /source_inv.
+    iMod (own_alloc (● (Excl' nil) ⋅ ◯ (Excl' nil))) as (γ2) "[Hauth Hfrag]".
+    { apply auth_both_valid; done. }
+    iApply (fupd_mask_weaken _ _).
+    { solve_ndisj. }
+    iExists l, nil. iFrame.
+    iSplitL "".
+    { iPureIntro; econstructor. }
+    iClear "Hctx Hinv".
+    iIntros (???) "(#Hctx&Hstate)".
+    rewrite /DBLockInv.
+    iModIntro. iExists _. iFrame. iExists γ2.
+    iSplitR "Hauth Hstate"; iIntros; iExists nil; iFrame.
+  Qed.
+
+  Lemma init_wf: ∀ σ1a σ1c, init_absr σ1a σ1c → ExMach.state_wf σ1c.
+  Proof. intros ?? (H&?). inversion H. subst. eapply ExMach.init_state_wf. Qed.
+
+  Lemma init_exec_inner : init_exec_inner_type.
+  Proof.
+    rewrite /init_exec_inner_type.
+    intros ?? (H&Hinit) ??. inversion H. inversion Hinit. subst.
+    iIntros "(Hmem&?&#?&Hstate)".
+    iMod (own_alloc (● (Excl' nil) ⋅ ◯ (Excl' nil))) as (γ2) "[Hauth Hfrag]".
+    { apply auth_both_valid. split; done. }
+    iPoseProof (init_mem_split with "Hmem") as "(?&?&?)".
+    iModIntro. iExists _. iFrame. iExists γ2. iSplitR "Hauth Hstate"; iIntros; iExists nil; iFrame.
+  Qed.
+
+  Lemma exec_inv_preserve_crash: exec_inv_preserve_crash_type.
+  Proof.
+    rewrite /exec_inv_preserve_crash_type.
+    intros. iIntros "(#Hctx&#Hinv)".
+    iDestruct "Hinv" as (γ1 γ2) "(Hlock&#Hinv)".
+    rewrite /DBCrashInner.
+    iInv "Hinv" as ">Hopen" "_".
+    iDestruct "Hopen" as (l) "(?&?)".
+    iApply fupd_mask_weaken; first by solve_ndisj.
+    iIntros (??) "Hmem".
+    iModIntro. iExists l; iFrame.
+    iPoseProof (@init_mem_split with "Hmem") as "(?&?&?)".
+    iFrame.
+  Qed.
+
+  Lemma crash_inv_preserve_crash: crash_inv_preserve_crash_type.
+  Proof.
+    rewrite /crash_inv_preserve_crash_type.
+    intros. iIntros "(#Hctx&#Hinv)".
+    rewrite /DBCrashInner.
+    iInv "Hinv" as ">Hopen" "_".
+    iDestruct "Hopen" as (l) "(?&?)".
+    iApply fupd_mask_weaken; first by solve_ndisj.
+    iIntros (??) "Hmem".
+    iModIntro. iExists l. iFrame.
+    iPoseProof (@init_mem_split with "Hmem") as "(?&?&?)".
+    iFrame.
+  Qed.
+
+  Lemma crash_inner_inv : crash_inner_inv_type.
+  Proof.
+    rewrite /crash_inner_inv_type.
+    intros. iIntros "H". iDestruct "H" as "(Hinv&#Hsrc)".
+    iDestruct "Hinv" as (invG) "Hinv".
+    rewrite /DBCrashInner/CrashInv.
+    iDestruct "Hinv" as (l) "(?&?)".
+    iMod (@inv_alloc Σ (exm_invG) iN _ DBCrashInner with "[-]").
+    { iNext. iExists l; iFrame. }
+    iModIntro. iFrame. iExists tt. iFrame "Hsrc".
+  Qed.
+
+  Lemma exec_inner_inv : exec_inner_inv_type.
+  Proof.
+    rewrite /exec_inner_inv_type.
+    intros. iIntros "H". iDestruct "H" as "(Hinv&#Hsrc)".
+    iDestruct "Hinv" as (invG v) "Hinv".
+    iDestruct "Hinv" as "(?&Hinv)".
+    iDestruct "Hinv" as (γ2) "(Hlock&Hinner)".
+    iMod (@lock_init Σ (ExMachG _ (exm_invG) (exm_mem_inG) (exm_disk_inG) _) _ lN
+                     lock_addr _ (DBLockInv γ2) with "[$] [-Hinner]") as (γ1) "H".
+    { iFrame. }
+    iMod (@inv_alloc Σ (exm_invG) iN _ (DBInnerInv γ2) with "[Hinner]").
+    { iFrame. }
+    iModIntro. rewrite /DBInv. iFrame "Hsrc". iExists γ1, γ2. iFrame.
+  Qed.
+
+  Lemma exec_inv_preserve_finish : exec_inv_preserve_finish_type.
+  Proof.
+    iIntros (??) "? (?&H)".
+    iDestruct "H" as (γ1 γ2) "(Hlock&Hinv)".
+    iInv "Hinv" as (l') ">(Htok&Hsource)" "_".
+    iMod (lock_crack with "Hlock") as ">H"; first by solve_ndisj.
+    iDestruct "H" as (v) "(?&?)".
+    iApply fupd_mask_weaken; first by solve_ndisj.
+    iExists _, nil; eauto.
+    iFrame. iSplitL ""; first by eauto.
+    iIntros (????) "(?&Hstate&Hmem)".
+    iPoseProof (@init_mem_split with "Hmem") as "(?&?&?)".
+    iMod (own_alloc (● (Excl' nil) ⋅ ◯ (Excl' nil))) as (γ2') "[Hauth Hfrag]".
+    { apply auth_both_valid. split; done. }
+    iModIntro. iExists O. iFrame.
+    iExists γ2'. rewrite /DBInnerInv/DBLockInv.
+    iSplitR "Hstate Hauth".
+    { iIntros. iExists _; iFrame. }
+    { iExists _; iFrame. }
+  Qed.
+
+End sRO.
+
+Module sR := exmach_refinement sRT sRO.
+Import sR.
+
+Lemma exmach_crash_refinement_seq {T} σ1c σ1a (es: proc_seq DB.Op T) :
+  sRT.init_absr σ1a σ1c →
+  wf_client_seq es →
+  ¬ proc_exec_seq DB.l es (rec_singleton (Ret ())) (1, σ1a) Err →
+  ∀ σ2c res, proc_exec_seq ExMach.l (compile_proc_seq StatDb.Impl.impl es)
+                                      (rec_singleton recv) (1, σ1c) (Val σ2c res) →
+  ∃ σ2a, proc_exec_seq DB.l es (rec_singleton (Ret tt)) (1, σ1a) (Val σ2a res).
+Proof. apply sR.R.crash_refinement_seq. Qed.
+
+Print Assumptions exmach_crash_refinement_seq.
